tmp

src/ChecksumLog.v
@@ -10,123 +10,170 @@ Require Import SepAuto2.
 Require Import Cache.
 Require Import Omega.
 Require Import GenSep.
+Require Import PredCrash.
 
 Set Implicit Arguments.
 
-Definition PreviousHash : addr := $0.
-Definition NextHash : addr := $1.
-Definition DataStart : addr := $2.
+Definition PreviousLength : addr := $0.
+Definition CurrentLength : addr := $1.
+Definition Checksum : addr := $2.
+Definition DataStart : addr := $3.
 Parameter maxlen : addr.
 
 Definition list_prefix A (p l : list A) :=
   firstn (length p) l = p.
 
-Definition log_rep_prefix h vl vdisk len hm :=
-  list_prefix vl vdisk /\
+Definition log_rep_prefix h len vl vdisk hm :=
   hash_list_rep (rev vl) h hm /\
-  length vdisk = len.
+  list_prefix vl vdisk /\
+  length vl = len.
 
-Definition log_rep vl vl' (log_pointer : addr) hm vdisk :
+(* EVentually len' can live in memory *)
+Definition log_rep vl vl' vdisk hm :
   @pred addr (@weq addrlen) valuset :=
-  (exists h h',
-    [[ log_rep_prefix h vl vl' # (log_pointer) hm ]] *
-    [[ log_rep_prefix h' vl' vdisk # (maxlen) hm ]] *
-    PreviousHash |-> (hash_to_valu h, nil) *
-    NextHash |-> (hash_to_valu h', nil) *
-    array DataStart (combine vdisk (repeat nil # (maxlen))) $1
+  (exists h h' len len',
+    [[ log_rep_prefix h len vl vl' hm ]] *
+    [[ log_rep_prefix h' len' vl' vdisk hm ]] *
+    [[ length vdisk = # (maxlen) ]] *
+    PreviousLength |-> (addr2valu $ (len), nil) *
+    CurrentLength |-> (addr2valu $ (len'), nil) *
+    Checksum |-> (hash_to_valu h', nil) *
+    array DataStart (combine vdisk (repeat nil # (maxlen))) $1)%pred.
+
+Definition crep vl vl' vl'' vdisk hm :
+  @pred addr (@weq addrlen) valuset :=
+  (exists h h' h'' len len' len'' unsynced_data,
+    [[ log_rep_prefix h len vl vl' hm ]] *
+    [[ log_rep_prefix h' len' vl' vl'' hm ]] *
+    [[ log_rep_prefix h'' len'' vl'' vdisk hm ]] *
+    (PreviousLength |-> (addr2valu $ (len), nil) \/
+      PreviousLength |-> (addr2valu $ (len'), addr2valu $ (len) :: nil)) *
+    (CurrentLength |-> (addr2valu $ (len'), nil) \/
+      CurrentLength |-> (addr2valu $ (len''), addr2valu $ (len') :: nil)) *
+    (Checksum |-> (hash_to_valu h', nil) \/
+      Checksum |-> (hash_to_valu h'', hash_to_valu h' :: nil)) *
+    (array DataStart (combine vdisk
+        (upd (repeat nil # (maxlen)) $ ( len') (unsynced_data :: nil))) $1)
   )%pred.
 
-(* What the rep *should* be after crash. *)
+(** What the rep *should* be after crash.
+- PreviousHash points to a synced hash value that matches a
+  prefix of the disk.
+- NextHash points to a synced hash value. If this hash matches
+  a prefix of the disk, then PreviousHash's matched disk prefix
+  is also a prefix of NextHash's disk prefix.
+- DataStart points to a synced array.
+
 Definition log_rep_part vl hm vdisk :
   @pred addr (@weq addrlen) valuset :=
   (exists h h',
     [[ log_rep_prefix h vl vdisk # (maxlen) hm ]] *
+    [[ (exists vl', log_rep_prefix h' vl' vdisk # (maxlen) hm
+        -> list_prefix vl vl') ]] *
     PreviousHash |-> (hash_to_valu h, nil) *
     NextHash |-> (hash_to_valu h', nil) *
     array DataStart (combine vdisk (repeat nil # (maxlen))) $1
-  )%pred.
+  )%pred.**)
 
-Definition log_rep' vl vl' log_pointer hm cs d : pred :=
+Definition log_rep' vl vl' hm cs d : pred :=
   BUFCACHE.rep cs d *
-  [[ (exists vdisk, log_rep vl vl' log_pointer hm vdisk)%pred d ]].
+  [[ (exists vdisk, log_rep vl vl' vdisk hm)%pred d ]].
 
-(**
-* - PreviousHash must be equal to either the previous hash, the next
-    hash, or the newest hash (hash of the value appended)
-  - PreviousHash must point to a hash that matches some prefix of
-    the current disk.
-* - NextHash can point to anything, as long as it's a hash value.
-* - Disk can have original log data, with possibility of log_pointer
-    position unsynced (only happens when when log_pointer hasn't been
-    incremented yet)
-**)
-Definition crep vl vl' (log_pointer : addr) hm vdisk :
-  @pred addr (@weq addrlen) valuset :=
-  (exists h h' unsynced_data,
-    [[ log_rep_prefix h vl vl' # (log_pointer) hm ]] *
-    [[ log_rep_prefix h' vl' vdisk # (maxlen) hm ]] *
-    (PreviousHash |-> (hash_to_valu h, nil) \/
-      PreviousHash |-> (hash_to_valu h', hash_to_valu h :: nil) \/
-      PreviousHash |-> (hash_to_valu h', nil)) *
-    (exists h' h'', NextHash |-> (hash_to_valu h'', nil) \/
-      NextHash |-> (hash_to_valu h'', hash_to_valu h' :: nil)) *
-    (array DataStart (combine vdisk
-        (upd (repeat nil # (maxlen)) log_pointer unsynced_data)) $1)
-  )%pred.
+Definition possible_crash_list (l: list valuset) (l': list valu) :=
+  length l = length l' /\ forall i, i < length l -> In (selN l' i $0) (valuset_list (selN l i ($0, nil))).
+
+Lemma crash_xform_array: forall l start stride,
+  crash_xform (array start l stride) =p=>
+    exists l', [[ possible_crash_list l l' ]] * array start (List.combine l' (repeat nil (length l'))) stride.
+Proof.
+Admitted.
+
+Lemma crash_invariant_synced_array: forall l start stride,
+  crash_xform (array start (List.combine l (repeat nil (length l))) stride) =p=>
+  array start (List.combine l (repeat nil (length l))) stride.
+Proof.
+Admitted.
+
+Lemma crash_xform_helper : forall vdisk log_pointer unsynced_data,
+  crash_xform (array DataStart (combine vdisk
+        (upd (repeat nil (length vdisk)) log_pointer (unsynced_data :: nil))) $1) =p=>
+    array DataStart (combine vdisk (repeat nil (length vdisk))) $1 \/
+    array DataStart (combine (upd vdisk log_pointer unsynced_data) (repeat nil (length vdisk))) $1.
+Proof.
+Admitted.
 
 Definition read T i (log_pointer : addr) cs rx : prog T :=
   let^ (cs, v) <- BUFCACHE.read_array DataStart i $1 cs;
   rx ^(cs, log_pointer, v).
 
-Definition append T v log_pointer cs rx : prog T :=
-  let^ (cs, h') <- BUFCACHE.read NextHash cs;
-  h'' <- Hash (Word.combine v (valu_to_hash h'));
-  cs <- BUFCACHE.write_array DataStart log_pointer $1 v cs;
-  cs <- BUFCACHE.write PreviousHash h' cs;
-  cs <- BUFCACHE.write NextHash (hash_to_valu h'') cs;
-  cs <- BUFCACHE.sync_array DataStart log_pointer $1 cs;
-  cs <- BUFCACHE.sync PreviousHash cs;
-  cs <- BUFCACHE.sync NextHash cs;
-  rx ^(cs, log_pointer ^+ $1).
+Definition append T v cs rx : prog T :=
+  let^ (cs, log_pointer) <- BUFCACHE.read CurrentLength cs;
+  let^ (cs, h) <- BUFCACHE.read Checksum cs;
+  h <- Hash (Word.combine v (valu_to_hash h));
+  cs <- BUFCACHE.write_array DataStart (valu2addr log_pointer) $1 v cs;
+  cs <- BUFCACHE.write PreviousLength log_pointer cs;
+  cs <- BUFCACHE.write CurrentLength (addr2valu (valu2addr log_pointer ^+ $1)) cs;
+  cs <- BUFCACHE.write Checksum (hash_to_valu h) cs;
+  cs <- BUFCACHE.sync_array DataStart (valu2addr log_pointer) $1 cs;
+  cs <- BUFCACHE.sync PreviousLength cs;
+  cs <- BUFCACHE.sync CurrentLength cs;
+  cs <- BUFCACHE.sync Checksum cs;
+  rx cs.
 
 Definition truncate T cs rx : prog T :=
   h <- Hash default_valu;
-  cs <- BUFCACHE.write PreviousHash (hash_to_valu h) cs;
-  cs <- BUFCACHE.write NextHash (hash_to_valu h) cs;
-  cs <- BUFCACHE.sync PreviousHash cs;
-  cs <- BUFCACHE.sync NextHash cs;
-  rx (cs, natToWord addrlen 0).
+  cs <- BUFCACHE.write PreviousLength $0 cs;
+  cs <- BUFCACHE.write CurrentLength $0 cs;
+  cs <- BUFCACHE.write Checksum (hash_to_valu h) cs;
+  cs <- BUFCACHE.sync PreviousLength cs;
+  cs <- BUFCACHE.sync CurrentLength cs;
+  cs <- BUFCACHE.sync Checksum cs;
+  rx cs.
 
-Theorem append_ok : forall log_pointer v cs,
+Theorem append_ok : forall v cs,
   {< d vl vl',
   PRE:hm
-    [[ # (log_pointer) < # (maxlen) ]] *
-    log_rep' vl vl' log_pointer hm cs d
-  POST:hm' RET:^(cs', log_pointer')
+    [[ length vl' < # (maxlen) ]] *
+    log_rep' vl vl' hm cs d
+  POST:hm' RET:cs'
     exists d',
-      log_rep' vl' (vl' ++ v :: nil) log_pointer' hm' cs' d'
+      log_rep' vl' (vl' ++ v :: nil) hm' cs' d'
   CRASH:hm'
-    exists cs' d' vdisk, BUFCACHE.rep cs' d' *
-      (crep vl vl' log_pointer hm' vdisk \/
-        crep vl' (vl' ++ v :: nil) (log_pointer ^+ $1) hm' vdisk)
-  >} append v log_pointer cs.
+    exists cs' d', BUFCACHE.rep cs' d' (** TODO **)
+  >} append v cs.
 Proof.
   unfold append, log_rep', log_rep, log_rep_prefix.
   step.
   pred_apply; cancel.
 
   step.
+  pred_apply; cancel.
   step.
-  admit. (* Solvable with list_prefix length lemma *)
+  step.
+  rewrite addr2valu2addr.
+  rewrite wordToNat_natToWord_bound with (bound := maxlen);
+    try omega.
+  rewrite combine_length.
+  rewrite repeat_length.
+  rewrite min_l; omega.
   step.
   pred_apply; cancel.
   step.
   pred_apply; cancel.
+  step.
+  pred_apply; cancel.
+
   step_idtac.
   eauto.
   pred_apply; cancel_with eauto.
-  instantiate (a25:=(upd_prepend (combine l (repeat nil # (maxlen))) log_pointer v)); cancel.
-  admit.
+  rewrite addr2valu2addr.
+  instantiate (a1:=(upd_prepend (combine l (repeat nil # (maxlen))) $ (length l1) v)); cancel.
+  rewrite addr2valu2addr.
+  rewrite wordToNat_natToWord_bound with (bound := maxlen);
+    try omega.
+  unfold upd_prepend.
+  rewrite length_upd, combine_length, repeat_length.
+  rewrite min_l; omega.
 
   step_idtac.
   eauto.
@@ -136,6 +183,11 @@ Proof.
   pred_apply; cancel_with eauto.
 
   step_idtac.
+  eauto.
+  pred_apply; cancel_with eauto.
+
+  step_idtac.
+
   Lemma upd_sync_prepend : forall l i v default,
     upd_sync (upd_prepend l i v) i default = upd l i (v, nil).
   Proof.
@@ -165,16 +217,17 @@ Proof.
     omega.
   Qed.
 
+  rewrite addr2valu2addr.
   rewrite upd_sync_prepend.
   rewrite <- combine_upd.
   rewrite repeat_upd.
   eauto.
 
+  solve_hash_list_rep.
   unfold list_prefix.
   apply firstn_app; auto.
-  solve_hash_list_rep.
-  admit.
-  admit. (* list_prefix holds for updated disk *)
+  rewrite wordToNat_natToWord_bound with (bound := maxlen);
+    try omega.
 
   rewrite rev_unit.
   econstructor.
@@ -184,14 +237,61 @@ Proof.
   eapply hashmap_get_subset.
   rewrite upd_hashmap'_eq. eauto.
   intuition.
-  rewrite H20 in H19.
+  rewrite H24 in H19.
   unfold hash_safe in H19; intuition.
-  contradict_hashmap_get_default H22 hm0.
-  contradict_hashmap_get_default H22 hm0.
-  instantiate (Goal:=hm0).
+  contradict_hashmap_get_default H26 hm1.
+  contradict_hashmap_get_default H26 hm1.
+  instantiate (Goal:=hm1).
   solve_hashmap_subset.
 
+  unfold list_prefix in H12.
+  unfold list_prefix.
+  unfold upd.
+  replace (length (l1 ++ _)) with (length l1 + 1).
+  rewrite wordToNat_natToWord_bound with (bound := maxlen);
+    try omega.
+  rewrite <- firstn_app_updN_eq.
+  congruence.
+  omega.
+  rewrite app_length; auto.
+  erewrite wordToNat_plusone.
+  rewrite wordToNat_natToWord_bound with (bound := maxlen);
+    try omega.
+  apply lt_wlt.
+  rewrite wordToNat_natToWord_bound with (bound := maxlen);
+    try omega.
+  eauto.
   rewrite length_upd; auto.
 
   (* creps... *)
-Admitted.
+  all: cancel_with eauto.
+Qed.
+
+Theorem truncate_ok : forall cs,
+  {< d vl vl',
+  PRE:hm
+    log_rep' vl vl' hm cs d
+  POST:hm' RET:cs'
+    exists d',
+      log_rep' nil nil hm' cs' d'
+  CRASH:hm'
+    exists cs' d', BUFCACHE.rep cs' d' (** TODO **)
+  >} truncate cs.
+Proof.
+  unfold truncate, log_rep', log_rep, log_rep_prefix.
+  step.
+  step.
+  step.
+  pred_apply; cancel.
+  step.
+  pred_apply; cancel.
+  step_idtac.
+  eauto.
+  pred_apply; cancel.
+  step_idtac.
+  eauto.
+  pred_apply; cancel.
+  step_idtac.
+  eauto.
+  pred_apply; cancel.
+  step.
